examples/dynamic_isolation/LogHelpers.v
@@ -1,5 +1,22 @@
 Require Import Koika.Frontend.
 
+Section LatestWrite.
+  Context {reg_t: Type}.
+  Context {R: reg_t -> type}.
+  Context {REnv: Env reg_t}.
+
+  Definition rew_latest_write0 {T} (log: Log R REnv) (reg: reg_t) (pf_R_equal: R reg = T) : option T :=
+    rew [fun t : type => option t] pf_R_equal in latest_write0 log reg.
+
+  Definition rew_latest_write1 {T} (log: Log R REnv) (reg: reg_t) (pf_R_equal: R reg = T) : option T :=
+    rew [fun t : type => option t] pf_R_equal in latest_write1 log reg.
+
+  Definition rew_latest_write {T} (log: Log R REnv) (reg: reg_t) (pf_R_equal: R reg = T) : option T :=
+    rew [fun t : type => option t] pf_R_equal in latest_write log reg.
+
+End LatestWrite.
+
+
 Section LogEvents.
   Context {reg_t: Type}.
   Context {R: reg_t -> type}.
@@ -10,7 +27,7 @@ Section LogEvents.
                               (log: Log R REnv) : option T :=
       match latest_write0 log valid_reg with
       | Some b => if Bits.single (rew [fun t : type => t] pf_R_valid_reg in b)
-                 then rew [fun t : type => option t] pf_R_data_reg in (latest_write0 log data_reg)
+                 then rew_latest_write0 log data_reg pf_R_data_reg
                  else None
       | None => None
       end.
@@ -20,9 +37,10 @@ Section LogEvents.
                               (log: Log R REnv) : option T :=
       match latest_write1 log valid_reg with
       | Some b => if Bits.single (rew [fun t : type => t] pf_R_valid_reg in b)
-                 then rew [fun t : type => option t] pf_R_data_reg in (latest_write1 log data_reg)
+                 then rew_latest_write1 log data_reg pf_R_data_reg
                  else None
       | None => None
       end.
 
 End LogEvents.
+
